abp/SenderAutomaton.thy
@@ -3,7 +3,7 @@
  * This file was generated from Sender.maa and will be overridden when changed. To change
  * permanently, consider changing the model itself.
  *
- * Generated on Sep 19, 2018 11:04:38 PM by isartransformer 1.0.0
+ * Generated on Sep 21, 2018 4:47:19 PM by isartransformer 1.0.0
  *)
 theory SenderAutomaton
   imports bundle.tsynBundle automat.dAutomaton
@@ -36,32 +36,21 @@ end
 
 section \<open>Helpers to create a bundle from a single raw element\<close>
 
-(* Create one sbElem for all input streams *)
-fun createSbElem_As_I :: "(bool tsyn) \<Rightarrow> (nat tsyn) \<Rightarrow> (senderMessage tsyn sbElem)" where
-"createSbElem_As_I null null = Abs_sbElem [\<C> ''as'' \<mapsto> null, \<C> ''i'' \<mapsto> null]" |
-"createSbElem_As_I (Msg port_as) null = Abs_sbElem [\<C> ''as'' \<mapsto> Msg (SenderBool port_as), \<C> ''i'' \<mapsto> null]" |
-"createSbElem_As_I null (Msg port_i) = Abs_sbElem [\<C> ''as'' \<mapsto> null, \<C> ''i'' \<mapsto> Msg (SenderNat port_i)]" |
-"createSbElem_As_I (Msg port_as) (Msg port_i) = Abs_sbElem [\<C> ''as'' \<mapsto> Msg (SenderBool port_as), \<C> ''i'' \<mapsto> Msg (SenderNat port_i)]"
-
-(* Create one SB for all input streams *)
-fun createBundle_As_I :: "(bool tsyn) \<Rightarrow> (nat tsyn) \<Rightarrow> (senderMessage tsyn SB)" where
-"createBundle_As_I port_as  port_i  = (sbe2SB (createSbElem_As_I port_as  port_i ))"
-
-lift_definition createAsBundle :: "bool \<Rightarrow> senderMessage tsyn sbElem" is
+lift_definition senderElem_raw_As :: "bool \<Rightarrow> senderMessage tsyn sbElem" is
 "\<lambda>x. [\<C> ''as'' \<mapsto> Msg (SenderBool x)]"
   unfolding sbElemWell_def
   unfolding usclOkay_stream_def
   unfolding ctype_tsyn_def
   by simp
 
-lift_definition createIBundle :: "nat \<Rightarrow> senderMessage tsyn sbElem" is
+lift_definition senderElem_raw_I :: "nat \<Rightarrow> senderMessage tsyn sbElem" is
 "\<lambda>x. [\<C> ''i'' \<mapsto> Msg (SenderNat x)]"
   unfolding sbElemWell_def
   unfolding usclOkay_stream_def
   unfolding ctype_tsyn_def
   by simp
 
-lift_definition createDsBundle :: "(nat\<times>bool) \<Rightarrow> senderMessage tsyn sbElem" is
+lift_definition senderElem_raw_Ds :: "(nat\<times>bool) \<Rightarrow> senderMessage tsyn sbElem" is
 "\<lambda>x. [\<C> ''ds'' \<mapsto> Msg (SenderPair_SenderNat_SenderBool x)]"
   unfolding sbElemWell_def
   unfolding usclOkay_stream_def
@@ -71,152 +60,108 @@ lift_definition createDsBundle :: "(nat\<times>bool) \<Rightarrow> senderMessage
 
 section \<open>Helpers to create a bundle from a single tsyn element\<close>
 
-fun createTsynAsBundle :: "bool tsyn \<Rightarrow> senderMessage tsyn SB" where
-"createTsynAsBundle (Msg x) = sbe2SB (createAsBundle x)" |
-"createTsynAsBundle null = sbe2SB (sbeNull {\<C> ''as''})"
+fun senderElem_As :: "bool tsyn \<Rightarrow> senderMessage tsyn sbElem" where
+"senderElem_As (Msg port_as) = senderElem_raw_As port_as" |
+"senderElem_As null = sbeNull {\<C> ''as''}"
 
-declare createTsynAsBundle.simps[simp del]
+definition sender_As :: "bool tsyn \<Rightarrow> senderMessage tsyn SB" where
+"sender_As port_as = sbe2SB (senderElem_As port_as)"
 
-fun createTsynIBundle :: "nat tsyn \<Rightarrow> senderMessage tsyn SB" where
-"createTsynIBundle (Msg x) = sbe2SB (createIBundle x)" |
-"createTsynIBundle null = sbe2SB (sbeNull {\<C> ''i''})"
+fun senderElem_I :: "nat tsyn \<Rightarrow> senderMessage tsyn sbElem" where
+"senderElem_I (Msg port_i) = senderElem_raw_I port_i" |
+"senderElem_I null = sbeNull {\<C> ''i''}"
 
-declare createTsynIBundle.simps[simp del]
+definition sender_I :: "nat tsyn \<Rightarrow> senderMessage tsyn SB" where
+"sender_I port_i = sbe2SB (senderElem_I port_i)"
 
-fun createTsynDsBundle :: "(nat\<times>bool) tsyn \<Rightarrow> senderMessage tsyn SB" where
-"createTsynDsBundle (Msg x) = sbe2SB (createDsBundle x)" |
-"createTsynDsBundle null = sbe2SB (sbeNull {\<C> ''ds''})"
+fun senderElem_Ds :: "(nat\<times>bool) tsyn \<Rightarrow> senderMessage tsyn sbElem" where
+"senderElem_Ds (Msg port_ds) = senderElem_raw_Ds port_ds" |
+"senderElem_Ds null = sbeNull {\<C> ''ds''}"
 
-declare createTsynDsBundle.simps[simp del]
+definition sender_Ds :: "(nat\<times>bool) tsyn \<Rightarrow> senderMessage tsyn SB" where
+"sender_Ds port_ds = sbe2SB (senderElem_Ds port_ds)"
+
+(* Create one sbElem for all input channels *)
+fun senderElemIn_As_I :: "bool tsyn \<Rightarrow> nat tsyn \<Rightarrow> senderMessage tsyn sbElem" where
+"senderElemIn_As_I port_as port_i = (senderElem_As port_as) \<plusminus> (senderElem_I port_i)"
+
+(* Create one sbElem for all output channels *)
+fun senderElemOut_Ds :: "(nat\<times>bool) tsyn \<Rightarrow> senderMessage tsyn sbElem" where
+"senderElemOut_Ds port_ds = (senderElem_Ds port_ds)"
+
+(* Create one SB for all input channels *)
+fun senderIn_As_I :: "bool tsyn \<Rightarrow> nat tsyn \<Rightarrow> senderMessage tsyn SB" where
+"senderIn_As_I port_as port_i = (sbe2SB (senderElemIn_As_I port_as port_i))"
+
+(* Create one SB for all output channels *)
+fun senderOut_Ds :: "(nat\<times>bool) tsyn \<Rightarrow> senderMessage tsyn SB" where
+"senderOut_Ds port_ds = (sbe2SB (senderElemOut_Ds port_ds))"
 
 
 section \<open>Helpers to create a bundle from a tsyn list of elements\<close>
 
-fun createLongAsBundle :: "(bool tsyn) list \<Rightarrow> senderMessage tsyn SB" where
-"createLongAsBundle (x#xs) = ubConcEq (createTsynAsBundle x)\<cdot>(createLongAsBundle xs)" |
-"createLongAsBundle []     = ubLeast {\<C> ''as''}"
+fun sender_list_As :: "(bool tsyn) list \<Rightarrow> senderMessage tsyn SB" where
+"sender_list_As (x#xs) = ubConcEq (sender_As x)\<cdot>(sender_list_As xs)" |
+"sender_list_As []     = ubLeast {\<C> ''as''}"
 
-fun createLongIBundle :: "(nat tsyn) list \<Rightarrow> senderMessage tsyn SB" where
-"createLongIBundle (x#xs) = ubConcEq (createTsynIBundle x)\<cdot>(createLongIBundle xs)" |
-"createLongIBundle []     = ubLeast {\<C> ''i''}"
+fun sender_list_I :: "(nat tsyn) list \<Rightarrow> senderMessage tsyn SB" where
+"sender_list_I (x#xs) = ubConcEq (sender_I x)\<cdot>(sender_list_I xs)" |
+"sender_list_I []     = ubLeast {\<C> ''i''}"
 
-fun createLongDsBundle :: "((nat\<times>bool) tsyn) list \<Rightarrow> senderMessage tsyn SB" where
-"createLongDsBundle (x#xs) = ubConcEq (createTsynDsBundle x)\<cdot>(createLongDsBundle xs)" |
-"createLongDsBundle []     = ubLeast {\<C> ''ds''}"
+fun sender_list_Ds :: "((nat\<times>bool) tsyn) list \<Rightarrow> senderMessage tsyn SB" where
+"sender_list_Ds (x#xs) = ubConcEq (sender_Ds x)\<cdot>(sender_list_Ds xs)" |
+"sender_list_Ds []     = ubLeast {\<C> ''ds''}"
 
+(* Create one SB for all input channels *)
+fun senderIn_list_As_I :: "bool tsyn list \<Rightarrow> nat tsyn list \<Rightarrow> senderMessage tsyn SB" where
+"senderIn_list_As_I port_as port_i = (sender_list_As port_as) \<uplus> (sender_list_I port_i)"
 
-section \<open>Lemmas for "createXBundle"\<close>
-
-lemma createAsBundle_dom [simp]: "sbeDom (createAsBundle x) = {\<C> ''as''}"
-  apply(simp add: sbeDom_def createAsBundle_def)
-  using createAsBundle.abs_eq createAsBundle.rep_eq by auto
-
-lemma createAsBundle_getch [simp]: "(sbe2SB (createAsBundle x)).(\<C> ''as'') = \<up>(Msg (SenderBool x))"
-  by (simp add: createAsBundle.rep_eq sbe2sb_getch)
-
-lemma createAsBundle_len [simp]: "ubLen (sbe2SB (createAsBundle x)) = Fin 1"
-  apply (subst ubLen_def)
-  apply (simp add: usclLen_stream_def)
-  by (metis (full_types) LeastI)
-
-lemma createIBundle_dom [simp]: "sbeDom (createIBundle x) = {\<C> ''i''}"
-  apply(simp add: sbeDom_def createIBundle_def)
-  using createIBundle.abs_eq createIBundle.rep_eq by auto
-
-lemma createIBundle_getch [simp]: "(sbe2SB (createIBundle x)).(\<C> ''i'') = \<up>(Msg (SenderNat x))"
-  by (simp add: createIBundle.rep_eq sbe2sb_getch)
-
-lemma createIBundle_len [simp]: "ubLen (sbe2SB (createIBundle x)) = Fin 1"
-  apply (subst ubLen_def)
-  apply (simp add: usclLen_stream_def)
-  by (metis (full_types) LeastI)
-
-lemma createDsBundle_dom [simp]: "sbeDom (createDsBundle x) = {\<C> ''ds''}"
-  apply(simp add: sbeDom_def createDsBundle_def)
-  using createDsBundle.abs_eq createDsBundle.rep_eq by auto
-
-lemma createDsBundle_getch [simp]: "(sbe2SB (createDsBundle x)).(\<C> ''ds'') = \<up>(Msg (SenderPair_SenderNat_SenderBool x))"
-  by (simp add: createDsBundle.rep_eq sbe2sb_getch)
-
-lemma createDsBundle_len [simp]: "ubLen (sbe2SB (createDsBundle x)) = Fin 1"
-  apply (subst ubLen_def)
-  apply (simp add: usclLen_stream_def)
-  by (metis (full_types) LeastI)
+(* Create one SB for all output channels *)
+fun senderOut_list_Ds :: "(nat\<times>bool) tsyn list \<Rightarrow> senderMessage tsyn SB" where
+"senderOut_list_Ds port_ds = (sender_list_Ds port_ds)"
 
 
-section \<open>Lemmas for "createTsynXBundle"\<close>
+section \<open>Helpers to create a bundle from a tsyn stream of elements\<close>
 
-lemma createTsynAsBundle_dom [simp]: "ubDom\<cdot>(createTsynAsBundle x) = {\<C> ''as''}"
-  by (cases x, simp_all add: createTsynAsBundle.simps)
+definition sender_stream_As :: "(bool) tsyn stream \<Rightarrow> senderMessage tsyn SB" where
+"sender_stream_As = undefined"
 
-lemma createTsynAsBundle_len [simp]: "ubLen (sbe2DB (createTsynAsBundle x)) = Fin 1"
-  apply (cases x, simp_all)
-  oops
+definition sender_stream_I :: "(nat) tsyn stream \<Rightarrow> senderMessage tsyn SB" where
+"sender_stream_I = undefined"
 
-lemma createTsynIBundle_dom [simp]: "ubDom\<cdot>(createTsynIBundle x) = {\<C> ''i''}"
-  by (cases x, simp_all add: createTsynIBundle.simps)
+definition sender_stream_Ds :: "((nat\<times>bool)) tsyn stream \<Rightarrow> senderMessage tsyn SB" where
+"sender_stream_Ds = undefined"
 
-lemma createTsynIBundle_len [simp]: "ubLen (sbe2DB (createTsynIBundle x)) = Fin 1"
-  apply (cases x, simp_all)
-  oops
+(* Create one SB for all input channels *)
+fun senderIn_stream_As_I :: "bool tsyn stream \<Rightarrow> nat tsyn stream \<Rightarrow> senderMessage tsyn SB" where
+"senderIn_stream_As_I port_as port_i = (sender_stream_As port_as) \<uplus> (sender_stream_I port_i)"
 
-lemma createTsynDsBundle_dom [simp]: "ubDom\<cdot>(createTsynDsBundle x) = {\<C> ''ds''}"
-  by (cases x, simp_all add: createTsynDsBundle.simps)
-
-lemma createTsynDsBundle_len [simp]: "ubLen (sbe2DB (createTsynDsBundle x)) = Fin 1"
-  apply (cases x, simp_all)
-  oops
+(* Create one SB for all output channels *)
+fun senderOut_stream_Ds :: "(nat\<times>bool) tsyn stream \<Rightarrow> senderMessage tsyn SB" where
+"senderOut_stream_Ds port_ds = (sender_stream_Ds port_ds)"
 
 
-section \<open>Lemmas for "createLongXBundle"\<close>
+section \<open>Helpers to get tsyn elements and streams from sbElems and SBs\<close>
 
-lemma createLongAsBundle_dom [simp]: "ubDom\<cdot>(createLongAsBundle xs) = {\<C> ''as''}"
-  proof (induction xs)
-    case Nil then show ?case by simp
-  next
-    case (Cons a _)
-      then show ?case
-        proof (cases a)
-          case (Msg _) then show ?thesis by (simp add: Cons.IH)
-        next
-          case null then show ?thesis by (simp add: Cons.IH)
-        qed
-  qed
+fun senderElem_get_As :: "senderMessage tsyn sbElem \<Rightarrow> (bool) tsyn" where
+"senderElem_get_As sbe = undefined"
 
-lemma createLongAsBundle_len [simp]: "ubLen (createLongAsBundle xs) = Fin (length xs)"
-  oops
+fun senderElem_get_stream_As :: "senderMessage tsyn SB \<Rightarrow> (bool) tsyn stream" where
+"senderElem_get_stream_As sb = undefined"
 
-lemma createLongIBundle_dom [simp]: "ubDom\<cdot>(createLongIBundle xs) = {\<C> ''i''}"
-  proof (induction xs)
-    case Nil then show ?case by simp
-  next
-    case (Cons a _)
-      then show ?case
-        proof (cases a)
-          case (Msg _) then show ?thesis by (simp add: Cons.IH)
-        next
-          case null then show ?thesis by (simp add: Cons.IH)
-        qed
-  qed
+fun senderElem_get_I :: "senderMessage tsyn sbElem \<Rightarrow> (nat) tsyn" where
+"senderElem_get_I sbe = undefined"
 
-lemma createLongIBundle_len [simp]: "ubLen (createLongIBundle xs) = Fin (length xs)"
-  oops
+fun senderElem_get_stream_I :: "senderMessage tsyn SB \<Rightarrow> (nat) tsyn stream" where
+"senderElem_get_stream_I sb = undefined"
 
-lemma createLongDsBundle_dom [simp]: "ubDom\<cdot>(createLongDsBundle xs) = {\<C> ''ds''}"
-  proof (induction xs)
-    case Nil then show ?case by simp
-  next
-    case (Cons a _)
-      then show ?case
-        proof (cases a)
-          case (Msg _) then show ?thesis by (simp add: Cons.IH)
-        next
-          case null then show ?thesis by (simp add: Cons.IH)
-        qed
-  qed
+fun senderElem_get_Ds :: "senderMessage tsyn sbElem \<Rightarrow> ((nat\<times>bool)) tsyn" where
+"senderElem_get_Ds sbe = undefined"
 
-lemma createLongDsBundle_len [simp]: "ubLen (createLongDsBundle xs) = Fin (length xs)"
-  oops
+fun senderElem_get_stream_Ds :: "senderMessage tsyn SB \<Rightarrow> ((nat\<times>bool)) tsyn stream" where
+"senderElem_get_stream_Ds sb = undefined"
+
+
 
 
 section \<open>Automaton definition\<close>
@@ -240,71 +185,79 @@ fun getC :: "SenderState \<Rightarrow> nat" where
 
 
 (* Helper that allows us to utilize pattern matching *)
-fun senderTransitionH :: "(SenderState \<times> (senderMessage tsyn \<times> senderMessage tsyn)) \<Rightarrow> (SenderState \<times> senderMessage tsyn SB)" where
-"senderTransitionH (SenderState Sf var_buffer var_c, (\<^cancel>\<open>as\<mapsto>\<close>Msg (SenderBool port_as), \<^cancel>\<open>i\<mapsto>\<close>Msg (SenderNat port_i))) =
-  (if((size var_buffer)>1 \<and> port_as=False) then ((SenderState St (prepend (butlast var_buffer) port_i) 3, (sbe2SB (createDsBundle (Pair (last (butlast var_buffer)) True)))))
-   else if((size var_buffer)=1 \<and> port_as=False) then ((SenderState St (prepend (butlast var_buffer) port_i) 3, (sbe2SB (createDsBundle (Pair port_i True)))))
-   else if((size var_buffer)=0) then ((SenderState Sf (prepend var_buffer port_i) 3, (sbe2SB (createDsBundle (Pair port_i False)))))
-   else if((size var_buffer)>0 \<and> var_c>0 \<and> port_as=True) then ((SenderState Sf (prepend var_buffer port_i) (var_c-1), (tsynbNull (\<C> ''ds''))))
-   else if((size var_buffer)>0 \<and> var_c=0 \<and> port_as=True) then ((SenderState Sf (prepend var_buffer port_i) 3, (sbe2SB (createDsBundle (Pair (last var_buffer) False)))))
-   else (SenderState Sf var_buffer var_c, (tsynbNull (\<C> ''ds''))))" |
+fun senderTransitionH :: "(SenderState \<times> (bool tsyn \<times> nat tsyn)) \<Rightarrow> (SenderState \<times> senderMessage tsyn SB)" where
+"senderTransitionH (SenderState Sf var_buffer var_c, (\<^cancel>\<open>as\<mapsto>\<close>Msg port_as, \<^cancel>\<open>i\<mapsto>\<close>Msg port_i)) =
+  (if((size var_buffer)>1 \<and> port_as=False) then ((SenderState St (prepend (butlast var_buffer) port_i) 3, (senderOut_Ds (Msg (Pair (last (butlast var_buffer)) True)))))
+   else if((size var_buffer)=1 \<and> port_as=False) then ((SenderState St (prepend (butlast var_buffer) port_i) 3, (senderOut_Ds (Msg (Pair port_i True)))))
+   else if((size var_buffer)=0) then ((SenderState Sf (prepend var_buffer port_i) 3, (senderOut_Ds (Msg (Pair port_i False)))))
+   else if((size var_buffer)>0 \<and> var_c>0 \<and> port_as=True) then ((SenderState Sf (prepend var_buffer port_i) (var_c-1), (senderOut_Ds null)))
+   else if((size var_buffer)>0 \<and> var_c=0 \<and> port_as=True) then ((SenderState Sf (prepend var_buffer port_i) 3, (senderOut_Ds (Msg (Pair (last var_buffer) False)))))
+   else (SenderState Sf var_buffer var_c, (senderOut_Ds null)))" |
 
-"senderTransitionH (SenderState Sf var_buffer var_c, (\<^cancel>\<open>as\<mapsto>\<close>Msg (SenderBool port_as), \<^cancel>\<open>i\<mapsto>\<close>null)) =
-  (if((size var_buffer)>1 \<and> port_as=False) then ((SenderState St (butlast var_buffer) 3, (sbe2SB (createDsBundle (Pair (last (butlast var_buffer)) True)))))
-   else if((size var_buffer)=1 \<and> port_as=False) then ((SenderState St (butlast var_buffer) var_c, (tsynbNull (\<C> ''ds''))))
-   else if((size var_buffer)=0) then ((SenderState Sf var_buffer var_c, (tsynbNull (\<C> ''ds''))))
-   else if((size var_buffer)>0 \<and> var_c>0 \<and> port_as=True) then ((SenderState Sf var_buffer (var_c-1), (tsynbNull (\<C> ''ds''))))
-   else if((size var_buffer)>0 \<and> var_c=0 \<and> port_as=True) then ((SenderState Sf var_buffer 3, (sbe2SB (createDsBundle (Pair (last var_buffer) False)))))
-   else (SenderState Sf var_buffer var_c, (tsynbNull (\<C> ''ds''))))" |
+"senderTransitionH (SenderState Sf var_buffer var_c, (\<^cancel>\<open>as\<mapsto>\<close>Msg port_as, \<^cancel>\<open>i\<mapsto>\<close>null)) =
+  (if((size var_buffer)>1 \<and> port_as=False) then ((SenderState St (butlast var_buffer) 3, (senderOut_Ds (Msg (Pair (last (butlast var_buffer)) True)))))
+   else if((size var_buffer)=1 \<and> port_as=False) then ((SenderState St (butlast var_buffer) var_c, (senderOut_Ds null)))
+   else if((size var_buffer)=0) then ((SenderState Sf var_buffer var_c, (senderOut_Ds null)))
+   else if((size var_buffer)>0 \<and> var_c>0 \<and> port_as=True) then ((SenderState Sf var_buffer (var_c-1), (senderOut_Ds null)))
+   else if((size var_buffer)>0 \<and> var_c=0 \<and> port_as=True) then ((SenderState Sf var_buffer 3, (senderOut_Ds (Msg (Pair (last var_buffer) False)))))
+   else (SenderState Sf var_buffer var_c, (senderOut_Ds null)))" |
 
-"senderTransitionH (SenderState Sf var_buffer var_c, (\<^cancel>\<open>as\<mapsto>\<close>null, \<^cancel>\<open>i\<mapsto>\<close>Msg (SenderNat port_i))) =
-  (if((size var_buffer)=0) then ((SenderState Sf (prepend var_buffer port_i) 3, (sbe2SB (createDsBundle (Pair port_i False)))))
-   else if((size var_buffer)>0 \<and> var_c>0) then ((SenderState Sf (prepend var_buffer port_i) (var_c-1), (tsynbNull (\<C> ''ds''))))
-   else if((size var_buffer)>0 \<and> var_c=0) then ((SenderState Sf (prepend var_buffer port_i) 3, (sbe2SB (createDsBundle (Pair (last var_buffer) False)))))
-   else (SenderState Sf var_buffer var_c, (tsynbNull (\<C> ''ds''))))" |
+"senderTransitionH (SenderState Sf var_buffer var_c, (\<^cancel>\<open>as\<mapsto>\<close>null, \<^cancel>\<open>i\<mapsto>\<close>Msg port_i)) =
+  (if((size var_buffer)=0) then ((SenderState Sf (prepend var_buffer port_i) 3, (senderOut_Ds (Msg (Pair port_i False)))))
+   else if((size var_buffer)>0 \<and> var_c>0) then ((SenderState Sf (prepend var_buffer port_i) (var_c-1), (senderOut_Ds null)))
+   else if((size var_buffer)>0 \<and> var_c=0) then ((SenderState Sf (prepend var_buffer port_i) 3, (senderOut_Ds (Msg (Pair (last var_buffer) False)))))
+   else (SenderState Sf var_buffer var_c, (senderOut_Ds null)))" |
 
 "senderTransitionH (SenderState Sf var_buffer var_c, (\<^cancel>\<open>as\<mapsto>\<close>null, \<^cancel>\<open>i\<mapsto>\<close>null)) =
-  (if((size var_buffer)=0) then ((SenderState Sf var_buffer var_c, (tsynbNull (\<C> ''ds''))))
-   else if((size var_buffer)>0 \<and> var_c>0) then ((SenderState Sf var_buffer var_c, (tsynbNull (\<C> ''ds''))))
-   else if((size var_buffer)>0 \<and> var_c=0) then ((SenderState Sf var_buffer 3, (sbe2SB (createDsBundle (Pair (last var_buffer) False)))))
-   else (SenderState Sf var_buffer var_c, (tsynbNull (\<C> ''ds''))))" |
+  (if((size var_buffer)=0) then ((SenderState Sf var_buffer var_c, (senderOut_Ds null)))
+   else if((size var_buffer)>0 \<and> var_c>0) then ((SenderState Sf var_buffer var_c, (senderOut_Ds null)))
+   else if((size var_buffer)>0 \<and> var_c=0) then ((SenderState Sf var_buffer 3, (senderOut_Ds (Msg (Pair (last var_buffer) False)))))
+   else (SenderState Sf var_buffer var_c, (senderOut_Ds null)))" |
 
-"senderTransitionH (SenderState St var_buffer var_c, (\<^cancel>\<open>as\<mapsto>\<close>Msg (SenderBool port_as), \<^cancel>\<open>i\<mapsto>\<close>Msg (SenderNat port_i))) =
-  (if((size var_buffer)=0) then ((SenderState St (prepend var_buffer port_i) 3, (sbe2SB (createDsBundle (Pair port_i True)))))
-   else if((size var_buffer)>1 \<and> port_as=True) then ((SenderState Sf (prepend (butlast var_buffer) port_i) 3, (sbe2SB (createDsBundle (Pair (last (butlast var_buffer)) False)))))
-   else if((size var_buffer)>0 \<and> var_c>0 \<and> port_as=False) then ((SenderState St (prepend var_buffer port_i) (var_c-1), (tsynbNull (\<C> ''ds''))))
-   else if((size var_buffer)>0 \<and> var_c=0 \<and> port_as=False) then ((SenderState St (prepend var_buffer port_i) 3, (sbe2SB (createDsBundle (Pair (last var_buffer) True)))))
-   else if((size var_buffer)=1 \<and> port_as=True) then ((SenderState Sf (prepend (butlast var_buffer) port_i) 3, (sbe2SB (createDsBundle (Pair port_i False)))))
-   else (SenderState St var_buffer var_c, (tsynbNull (\<C> ''ds''))))" |
+"senderTransitionH (SenderState St var_buffer var_c, (\<^cancel>\<open>as\<mapsto>\<close>Msg port_as, \<^cancel>\<open>i\<mapsto>\<close>Msg port_i)) =
+  (if((size var_buffer)=0) then ((SenderState St (prepend var_buffer port_i) 3, (senderOut_Ds (Msg (Pair port_i True)))))
+   else if((size var_buffer)>1 \<and> port_as=True) then ((SenderState Sf (prepend (butlast var_buffer) port_i) 3, (senderOut_Ds (Msg (Pair (last (butlast var_buffer)) False)))))
+   else if((size var_buffer)>0 \<and> var_c>0 \<and> port_as=False) then ((SenderState St (prepend var_buffer port_i) (var_c-1), (senderOut_Ds null)))
+   else if((size var_buffer)>0 \<and> var_c=0 \<and> port_as=False) then ((SenderState St (prepend var_buffer port_i) 3, (senderOut_Ds (Msg (Pair (last var_buffer) True)))))
+   else if((size var_buffer)=1 \<and> port_as=True) then ((SenderState Sf (prepend (butlast var_buffer) port_i) 3, (senderOut_Ds (Msg (Pair port_i False)))))
+   else (SenderState St var_buffer var_c, (senderOut_Ds null)))" |
 
-"senderTransitionH (SenderState St var_buffer var_c, (\<^cancel>\<open>as\<mapsto>\<close>Msg (SenderBool port_as), \<^cancel>\<open>i\<mapsto>\<close>null)) =
-  (if((size var_buffer)=0) then ((SenderState St var_buffer var_c, (tsynbNull (\<C> ''ds''))))
-   else if((size var_buffer)>1 \<and> port_as=True) then ((SenderState Sf (butlast var_buffer) 3, (sbe2SB (createDsBundle (Pair (last (butlast var_buffer)) False)))))
-   else if((size var_buffer)>0 \<and> var_c>0 \<and> port_as=False) then ((SenderState St var_buffer (var_c-1), (tsynbNull (\<C> ''ds''))))
-   else if((size var_buffer)>0 \<and> var_c=0 \<and> port_as=False) then ((SenderState St var_buffer 3, (sbe2SB (createDsBundle (Pair (last var_buffer) True)))))
-   else if((size var_buffer)=1 \<and> port_as=True) then ((SenderState Sf (butlast var_buffer) var_c, (tsynbNull (\<C> ''ds''))))
-   else (SenderState St var_buffer var_c, (tsynbNull (\<C> ''ds''))))" |
+"senderTransitionH (SenderState St var_buffer var_c, (\<^cancel>\<open>as\<mapsto>\<close>Msg port_as, \<^cancel>\<open>i\<mapsto>\<close>null)) =
+  (if((size var_buffer)=0) then ((SenderState St var_buffer var_c, (senderOut_Ds null)))
+   else if((size var_buffer)>1 \<and> port_as=True) then ((SenderState Sf (butlast var_buffer) 3, (senderOut_Ds (Msg (Pair (last (butlast var_buffer)) False)))))
+   else if((size var_buffer)>0 \<and> var_c>0 \<and> port_as=False) then ((SenderState St var_buffer (var_c-1), (senderOut_Ds null)))
+   else if((size var_buffer)>0 \<and> var_c=0 \<and> port_as=False) then ((SenderState St var_buffer 3, (senderOut_Ds (Msg (Pair (last var_buffer) True)))))
+   else if((size var_buffer)=1 \<and> port_as=True) then ((SenderState Sf (butlast var_buffer) var_c, (senderOut_Ds null)))
+   else (SenderState St var_buffer var_c, (senderOut_Ds null)))" |
 
-"senderTransitionH (SenderState St var_buffer var_c, (\<^cancel>\<open>as\<mapsto>\<close>null, \<^cancel>\<open>i\<mapsto>\<close>Msg (SenderNat port_i))) =
-  (if((size var_buffer)=0) then ((SenderState St (prepend var_buffer port_i) 3, (sbe2SB (createDsBundle (Pair port_i True)))))
-   else if((size var_buffer)>0 \<and> var_c>0) then ((SenderState St (prepend var_buffer port_i) (var_c-1), (tsynbNull (\<C> ''ds''))))
-   else if((size var_buffer)>0 \<and> var_c=0) then ((SenderState St (prepend var_buffer port_i) 3, (sbe2SB (createDsBundle (Pair (last var_buffer) True)))))
-   else (SenderState St var_buffer var_c, (tsynbNull (\<C> ''ds''))))" |
+"senderTransitionH (SenderState St var_buffer var_c, (\<^cancel>\<open>as\<mapsto>\<close>null, \<^cancel>\<open>i\<mapsto>\<close>Msg port_i)) =
+  (if((size var_buffer)=0) then ((SenderState St (prepend var_buffer port_i) 3, (senderOut_Ds (Msg (Pair port_i True)))))
+   else if((size var_buffer)>0 \<and> var_c>0) then ((SenderState St (prepend var_buffer port_i) (var_c-1), (senderOut_Ds null)))
+   else if((size var_buffer)>0 \<and> var_c=0) then ((SenderState St (prepend var_buffer port_i) 3, (senderOut_Ds (Msg (Pair (last var_buffer) True)))))
+   else (SenderState St var_buffer var_c, (senderOut_Ds null)))" |
 
 "senderTransitionH (SenderState St var_buffer var_c, (\<^cancel>\<open>as\<mapsto>\<close>null, \<^cancel>\<open>i\<mapsto>\<close>null)) =
-  (if((size var_buffer)=0) then ((SenderState St var_buffer var_c, (tsynbNull (\<C> ''ds''))))
-   else if((size var_buffer)>0 \<and> var_c>0) then ((SenderState St var_buffer (var_c-1), (tsynbNull (\<C> ''ds''))))
-   else if((size var_buffer)>0 \<and> var_c=0) then ((SenderState St var_buffer 3, (sbe2SB (createDsBundle (Pair (last var_buffer) True)))))
-   else (SenderState St var_buffer var_c, (tsynbNull (\<C> ''ds''))))"
+  (if((size var_buffer)=0) then ((SenderState St var_buffer var_c, (senderOut_Ds null)))
+   else if((size var_buffer)>0 \<and> var_c>0) then ((SenderState St var_buffer (var_c-1), (senderOut_Ds null)))
+   else if((size var_buffer)>0 \<and> var_c=0) then ((SenderState St var_buffer 3, (senderOut_Ds (Msg (Pair (last var_buffer) True)))))
+   else (SenderState St var_buffer var_c, (senderOut_Ds null)))"
+
+(* Domain *)
+definition senderDom :: "channel set" where
+"senderDom = {\<C> ''as'', \<C> ''i''}"
+
+(* Range *)
+definition senderRan :: "channel set" where
+"senderRan = {\<C> ''ds''}"
 
 (* Transition function *)
 fun senderTransition :: "(SenderState \<times> senderMessage tsyn sbElem) \<Rightarrow> (SenderState \<times> senderMessage tsyn SB)" where
-"senderTransition (s,b) = (if (sbeDom b) = {\<C> ''as'', \<C> ''i''} then senderTransitionH (s, (Rep_sbElem b\<rightharpoonup>\<C> ''as'', Rep_sbElem b\<rightharpoonup>\<C> ''i'')) else undefined)"
+"senderTransition (s,b) = (if (sbeDom b) = senderDom then senderTransitionH (s, (senderElem_get_As b, senderElem_get_I b)) else undefined)"
 
 (* The final automaton *)
 lift_definition SenderAutomaton :: "(SenderState, senderMessage tsyn) dAutomaton" is
-"(senderTransition, SenderState St []  0, tsynbNull (\<C> ''ds''), {\<C> ''as'', \<C> ''i''}, {\<C> ''ds''})"
-  by simp
+"(senderTransition, SenderState St []  0, (senderOut_Ds null), senderDom, senderRan)"
+  by (simp add: senderDom_def senderRan_def)
 
 (* Stream processing function for each state (handy for step lemmata) *)
 definition SenderStep :: "(SenderState \<Rightarrow> (senderMessage tsyn, senderMessage tsyn) SPF)" where
@@ -320,225 +273,225 @@ section \<open>Step-wise lemmata for the transition function\<close>
 (* Line 33:  Sf -> St [buffer.size()>1 && i!=null] {as==false} / {buffer=buffer.butlast().prepend(i), c=3, ds=new Pair<>(buffer.butlast().last(),true)}; *)
 lemma transition_0_0:
   assumes "(size var_buffer)>1 \<and> port_as=False"
-    shows "senderTransition ((SenderState Sf var_buffer var_c), (createSbElem_As_I (Msg port_as) (Msg port_i)))
-         = (SenderState St (prepend (butlast var_buffer) port_i) 3, (sbe2SB (createDsBundle (Pair (last (butlast var_buffer)) True))))"
+    shows "senderTransition ((SenderState Sf var_buffer var_c), (senderElemIn_As_I (Msg port_as) (Msg port_i)))
+         = (SenderState St (prepend (butlast var_buffer) port_i) 3, (senderOut_Ds (Msg (Pair (last (butlast var_buffer)) True))))"
   oops
 
 (* Line 35:  Sf -> St [buffer.size()=1 && i!=null] {as==false} / {buffer=buffer.butlast().prepend(i), c=3, ds=new Pair<>(i,true)}; *)
 lemma transition_0_1:
   assumes "(size var_buffer)=1 \<and> port_as=False"
-    shows "senderTransition ((SenderState Sf var_buffer var_c), (createSbElem_As_I (Msg port_as) (Msg port_i)))
-         = (SenderState St (prepend (butlast var_buffer) port_i) 3, (sbe2SB (createDsBundle (Pair port_i True))))"
+    shows "senderTransition ((SenderState Sf var_buffer var_c), (senderElemIn_As_I (Msg port_as) (Msg port_i)))
+         = (SenderState St (prepend (butlast var_buffer) port_i) 3, (senderOut_Ds (Msg (Pair port_i True))))"
   oops
 
 (* Line 43:  Sf -> Sf [buffer.size()=0 && as!=null && i!=null] / {buffer=buffer.prepend(i), c=3, ds=new Pair<>(i,false)}; *)
 lemma transition_0_2:
   assumes "(size var_buffer)=0"
-    shows "senderTransition ((SenderState Sf var_buffer var_c), (createSbElem_As_I (Msg port_as) (Msg port_i)))
-         = (SenderState Sf (prepend var_buffer port_i) 3, (sbe2SB (createDsBundle (Pair port_i False))))"
+    shows "senderTransition ((SenderState Sf var_buffer var_c), (senderElemIn_As_I (Msg port_as) (Msg port_i)))
+         = (SenderState Sf (prepend var_buffer port_i) 3, (senderOut_Ds (Msg (Pair port_i False))))"
   oops
 
 (* Line 45:  Sf -> Sf [buffer.size()>0 && c>0 && i!=null] {as==true} / {buffer=buffer.prepend(i), c=c-1}; *)
 lemma transition_0_3:
   assumes "(size var_buffer)>0 \<and> var_c>0 \<and> port_as=True"
-    shows "senderTransition ((SenderState Sf var_buffer var_c), (createSbElem_As_I (Msg port_as) (Msg port_i)))
-         = (SenderState Sf (prepend var_buffer port_i) (var_c-1), (tsynbNull (\<C> ''ds'')))"
+    shows "senderTransition ((SenderState Sf var_buffer var_c), (senderElemIn_As_I (Msg port_as) (Msg port_i)))
+         = (SenderState Sf (prepend var_buffer port_i) (var_c-1), (senderOut_Ds null))"
   oops
 
 (* Line 47:  Sf -> Sf [buffer.size()>0 && c=0 && i!=null] {as==true} / {buffer=buffer.prepend(i), c=3, ds=new Pair<>(buffer.last(),false)}; *)
 lemma transition_0_4:
   assumes "(size var_buffer)>0 \<and> var_c=0 \<and> port_as=True"
-    shows "senderTransition ((SenderState Sf var_buffer var_c), (createSbElem_As_I (Msg port_as) (Msg port_i)))
-         = (SenderState Sf (prepend var_buffer port_i) 3, (sbe2SB (createDsBundle (Pair (last var_buffer) False))))"
+    shows "senderTransition ((SenderState Sf var_buffer var_c), (senderElemIn_As_I (Msg port_as) (Msg port_i)))
+         = (SenderState Sf (prepend var_buffer port_i) 3, (senderOut_Ds (Msg (Pair (last var_buffer) False))))"
   oops
 
 (* Line 34:  Sf -> St [buffer.size()>1] {as==false, i==null} / {buffer=buffer.butlast(), c=3, ds=new Pair<>(buffer.butlast().last(),true)}; *)
 lemma transition_1_0:
   assumes "(size var_buffer)>1 \<and> port_as=False"
-    shows "senderTransition ((SenderState Sf var_buffer var_c), (createSbElem_As_I (Msg port_as) null))
-         = (SenderState St (butlast var_buffer) 3, (sbe2SB (createDsBundle (Pair (last (butlast var_buffer)) True))))"
+    shows "senderTransition ((SenderState Sf var_buffer var_c), (senderElemIn_As_I (Msg port_as) null))
+         = (SenderState St (butlast var_buffer) 3, (senderOut_Ds (Msg (Pair (last (butlast var_buffer)) True))))"
   oops
 
 (* Line 36:  Sf -> St [buffer.size()=1] {as==false, i==null} / {buffer=buffer.butlast()}; *)
 lemma transition_1_1:
   assumes "(size var_buffer)=1 \<and> port_as=False"
-    shows "senderTransition ((SenderState Sf var_buffer var_c), (createSbElem_As_I (Msg port_as) null))
-         = (SenderState St (butlast var_buffer) var_c, (tsynbNull (\<C> ''ds'')))"
+    shows "senderTransition ((SenderState Sf var_buffer var_c), (senderElemIn_As_I (Msg port_as) null))
+         = (SenderState St (butlast var_buffer) var_c, (senderOut_Ds null))"
   oops
 
 (* Line 38:  Sf -> Sf [buffer.size()=0 && as!=null] {i==null}; *)
 lemma transition_1_2:
   assumes "(size var_buffer)=0"
-    shows "senderTransition ((SenderState Sf var_buffer var_c), (createSbElem_As_I (Msg port_as) null))
-         = (SenderState Sf var_buffer var_c, (tsynbNull (\<C> ''ds'')))"
+    shows "senderTransition ((SenderState Sf var_buffer var_c), (senderElemIn_As_I (Msg port_as) null))
+         = (SenderState Sf var_buffer var_c, (senderOut_Ds null))"
   oops
 
 (* Line 40:  Sf -> Sf [buffer.size()>0 && c>0] {as==true, i==null} / {c=c-1}; *)
 lemma transition_1_3:
   assumes "(size var_buffer)>0 \<and> var_c>0 \<and> port_as=True"
-    shows "senderTransition ((SenderState Sf var_buffer var_c), (createSbElem_As_I (Msg port_as) null))
-         = (SenderState Sf var_buffer (var_c-1), (tsynbNull (\<C> ''ds'')))"
+    shows "senderTransition ((SenderState Sf var_buffer var_c), (senderElemIn_As_I (Msg port_as) null))
+         = (SenderState Sf var_buffer (var_c-1), (senderOut_Ds null))"
   oops
 
 (* Line 41:  Sf -> Sf [buffer.size()>0 && c=0] {as==true, i==null} / {c=3, ds=new Pair<>(buffer.last(),false)}; *)
 lemma transition_1_4:
   assumes "(size var_buffer)>0 \<and> var_c=0 \<and> port_as=True"
-    shows "senderTransition ((SenderState Sf var_buffer var_c), (createSbElem_As_I (Msg port_as) null))
-         = (SenderState Sf var_buffer 3, (sbe2SB (createDsBundle (Pair (last var_buffer) False))))"
+    shows "senderTransition ((SenderState Sf var_buffer var_c), (senderElemIn_As_I (Msg port_as) null))
+         = (SenderState Sf var_buffer 3, (senderOut_Ds (Msg (Pair (last var_buffer) False))))"
   oops
 
 (* Line 44:  Sf -> Sf [buffer.size()=0 && i!=null] {as==null} / {buffer=buffer.prepend(i), c=3, ds=new Pair<>(i,false)}; *)
 lemma transition_2_0:
   assumes "(size var_buffer)=0"
-    shows "senderTransition ((SenderState Sf var_buffer var_c), (createSbElem_As_I null (Msg port_i)))
-         = (SenderState Sf (prepend var_buffer port_i) 3, (sbe2SB (createDsBundle (Pair port_i False))))"
+    shows "senderTransition ((SenderState Sf var_buffer var_c), (senderElemIn_As_I null (Msg port_i)))
+         = (SenderState Sf (prepend var_buffer port_i) 3, (senderOut_Ds (Msg (Pair port_i False))))"
   oops
 
 (* Line 46:  Sf -> Sf [buffer.size()>0 && c>0 && i!=null] {as==null} / {buffer=buffer.prepend(i), c=c-1}; *)
 lemma transition_2_1:
   assumes "(size var_buffer)>0 \<and> var_c>0"
-    shows "senderTransition ((SenderState Sf var_buffer var_c), (createSbElem_As_I null (Msg port_i)))
-         = (SenderState Sf (prepend var_buffer port_i) (var_c-1), (tsynbNull (\<C> ''ds'')))"
+    shows "senderTransition ((SenderState Sf var_buffer var_c), (senderElemIn_As_I null (Msg port_i)))
+         = (SenderState Sf (prepend var_buffer port_i) (var_c-1), (senderOut_Ds null))"
   oops
 
 (* Line 48:  Sf -> Sf [buffer.size()>0 && c=0 && i!=null] {as==null} / {buffer=buffer.prepend(i), c=3, ds=new Pair<>(buffer.last(),false)}; *)
 lemma transition_2_2:
   assumes "(size var_buffer)>0 \<and> var_c=0"
-    shows "senderTransition ((SenderState Sf var_buffer var_c), (createSbElem_As_I null (Msg port_i)))
-         = (SenderState Sf (prepend var_buffer port_i) 3, (sbe2SB (createDsBundle (Pair (last var_buffer) False))))"
+    shows "senderTransition ((SenderState Sf var_buffer var_c), (senderElemIn_As_I null (Msg port_i)))
+         = (SenderState Sf (prepend var_buffer port_i) 3, (senderOut_Ds (Msg (Pair (last var_buffer) False))))"
   oops
 
 (* Line 37:  Sf -> Sf [buffer.size()=0] {as==null, i==null}; *)
 lemma transition_3_0:
   assumes "(size var_buffer)=0"
-    shows "senderTransition ((SenderState Sf var_buffer var_c), (createSbElem_As_I null null))
-         = (SenderState Sf var_buffer var_c, (tsynbNull (\<C> ''ds'')))"
+    shows "senderTransition ((SenderState Sf var_buffer var_c), (senderElemIn_As_I null null))
+         = (SenderState Sf var_buffer var_c, (senderOut_Ds null))"
   oops
 
 (* Line 39:  Sf -> Sf [buffer.size()>0 && c>0] {as==null, i==null}; *)
 lemma transition_3_1:
   assumes "(size var_buffer)>0 \<and> var_c>0"
-    shows "senderTransition ((SenderState Sf var_buffer var_c), (createSbElem_As_I null null))
-         = (SenderState Sf var_buffer var_c, (tsynbNull (\<C> ''ds'')))"
+    shows "senderTransition ((SenderState Sf var_buffer var_c), (senderElemIn_As_I null null))
+         = (SenderState Sf var_buffer var_c, (senderOut_Ds null))"
   oops
 
 (* Line 42:  Sf -> Sf [buffer.size()>0 && c=0] {as==null, i==null} / {c=3, ds=new Pair<>(buffer.last(),false)}; *)
 lemma transition_3_2:
   assumes "(size var_buffer)>0 \<and> var_c=0"
-    shows "senderTransition ((SenderState Sf var_buffer var_c), (createSbElem_As_I null null))
-         = (SenderState Sf var_buffer 3, (sbe2SB (createDsBundle (Pair (last var_buffer) False))))"
+    shows "senderTransition ((SenderState Sf var_buffer var_c), (senderElemIn_As_I null null))
+         = (SenderState Sf var_buffer 3, (senderOut_Ds (Msg (Pair (last var_buffer) False))))"
   oops
 
 (* Line 25:  St -> St [buffer.size()=0 && as!=null && i!=null] / {buffer=buffer.prepend(i), c=3, ds=new Pair<>(i,true)}; *)
 lemma transition_4_0:
   assumes "(size var_buffer)=0"
-    shows "senderTransition ((SenderState St var_buffer var_c), (createSbElem_As_I (Msg port_as) (Msg port_i)))
-         = (SenderState St (prepend var_buffer port_i) 3, (sbe2SB (createDsBundle (Pair port_i True))))"
+    shows "senderTransition ((SenderState St var_buffer var_c), (senderElemIn_As_I (Msg port_as) (Msg port_i)))
+         = (SenderState St (prepend var_buffer port_i) 3, (senderOut_Ds (Msg (Pair port_i True))))"
   oops
 
 (* Line 27:  St -> Sf [buffer.size()>1 && i!=null] {as==true} / {buffer=buffer.butlast().prepend(i), c=3, ds=new Pair<>(buffer.butlast().last(),false)}; *)
 lemma transition_4_1:
   assumes "(size var_buffer)>1 \<and> port_as=True"
-    shows "senderTransition ((SenderState St var_buffer var_c), (createSbElem_As_I (Msg port_as) (Msg port_i)))
-         = (SenderState Sf (prepend (butlast var_buffer) port_i) 3, (sbe2SB (createDsBundle (Pair (last (butlast var_buffer)) False))))"
+    shows "senderTransition ((SenderState St var_buffer var_c), (senderElemIn_As_I (Msg port_as) (Msg port_i)))
+         = (SenderState Sf (prepend (butlast var_buffer) port_i) 3, (senderOut_Ds (Msg (Pair (last (butlast var_buffer)) False))))"
   oops
 
 (* Line 28:  St -> St [buffer.size()>0 && c>0 && i!=null] {as==false} / {buffer=buffer.prepend(i), c=c-1}; *)
 lemma transition_4_2:
   assumes "(size var_buffer)>0 \<and> var_c>0 \<and> port_as=False"
-    shows "senderTransition ((SenderState St var_buffer var_c), (createSbElem_As_I (Msg port_as) (Msg port_i)))
-         = (SenderState St (prepend var_buffer port_i) (var_c-1), (tsynbNull (\<C> ''ds'')))"
+    shows "senderTransition ((SenderState St var_buffer var_c), (senderElemIn_As_I (Msg port_as) (Msg port_i)))
+         = (SenderState St (prepend var_buffer port_i) (var_c-1), (senderOut_Ds null))"
   oops
 
 (* Line 30:  St -> St [buffer.size()>0 && c=0 && i!=null] {as==false} / {buffer=buffer.prepend(i), c=3, ds=new Pair<>(buffer.last(),true)}; *)
 lemma transition_4_3:
   assumes "(size var_buffer)>0 \<and> var_c=0 \<and> port_as=False"
-    shows "senderTransition ((SenderState St var_buffer var_c), (createSbElem_As_I (Msg port_as) (Msg port_i)))
-         = (SenderState St (prepend var_buffer port_i) 3, (sbe2SB (createDsBundle (Pair (last var_buffer) True))))"
+    shows "senderTransition ((SenderState St var_buffer var_c), (senderElemIn_As_I (Msg port_as) (Msg port_i)))
+         = (SenderState St (prepend var_buffer port_i) 3, (senderOut_Ds (Msg (Pair (last var_buffer) True))))"
   oops
 
 (* Line 32:  St -> Sf [buffer.size()=1 && i!=null] {as==true} / {buffer=buffer.butlast().prepend(i), c=3, ds=new Pair<>(i,false)}; *)
 lemma transition_4_4:
   assumes "(size var_buffer)=1 \<and> port_as=True"
-    shows "senderTransition ((SenderState St var_buffer var_c), (createSbElem_As_I (Msg port_as) (Msg port_i)))
-         = (SenderState Sf (prepend (butlast var_buffer) port_i) 3, (sbe2SB (createDsBundle (Pair port_i False))))"
+    shows "senderTransition ((SenderState St var_buffer var_c), (senderElemIn_As_I (Msg port_as) (Msg port_i)))
+         = (SenderState Sf (prepend (butlast var_buffer) port_i) 3, (senderOut_Ds (Msg (Pair port_i False))))"
   oops
 
 (* Line 17:  St -> St [buffer.size()=0 && as!=null] {i==null}; *)
 lemma transition_5_0:
   assumes "(size var_buffer)=0"
-    shows "senderTransition ((SenderState St var_buffer var_c), (createSbElem_As_I (Msg port_as) null))
-         = (SenderState St var_buffer var_c, (tsynbNull (\<C> ''ds'')))"
+    shows "senderTransition ((SenderState St var_buffer var_c), (senderElemIn_As_I (Msg port_as) null))
+         = (SenderState St var_buffer var_c, (senderOut_Ds null))"
   oops
 
 (* Line 18:  St -> Sf [buffer.size()>1] {as==true, i==null} / {buffer=buffer.butlast(), c=3, ds=new Pair<>(buffer.butlast().last(),false)}; *)
 lemma transition_5_1:
   assumes "(size var_buffer)>1 \<and> port_as=True"
-    shows "senderTransition ((SenderState St var_buffer var_c), (createSbElem_As_I (Msg port_as) null))
-         = (SenderState Sf (butlast var_buffer) 3, (sbe2SB (createDsBundle (Pair (last (butlast var_buffer)) False))))"
+    shows "senderTransition ((SenderState St var_buffer var_c), (senderElemIn_As_I (Msg port_as) null))
+         = (SenderState Sf (butlast var_buffer) 3, (senderOut_Ds (Msg (Pair (last (butlast var_buffer)) False))))"
   oops
 
 (* Line 20:  St -> St [buffer.size()>0 && c>0] {as==false, i==null} / {c=c-1}; *)
 lemma transition_5_2:
   assumes "(size var_buffer)>0 \<and> var_c>0 \<and> port_as=False"
-    shows "senderTransition ((SenderState St var_buffer var_c), (createSbElem_As_I (Msg port_as) null))
-         = (SenderState St var_buffer (var_c-1), (tsynbNull (\<C> ''ds'')))"
+    shows "senderTransition ((SenderState St var_buffer var_c), (senderElemIn_As_I (Msg port_as) null))
+         = (SenderState St var_buffer (var_c-1), (senderOut_Ds null))"
   oops
 
 (* Line 22:  St -> St [buffer.size()>0 && c=0] {as==false, i==null} / {c=3, ds=new Pair<>(buffer.last(),true)}; *)
 lemma transition_5_3:
   assumes "(size var_buffer)>0 \<and> var_c=0 \<and> port_as=False"
-    shows "senderTransition ((SenderState St var_buffer var_c), (createSbElem_As_I (Msg port_as) null))
-         = (SenderState St var_buffer 3, (sbe2SB (createDsBundle (Pair (last var_buffer) True))))"
+    shows "senderTransition ((SenderState St var_buffer var_c), (senderElemIn_As_I (Msg port_as) null))
+         = (SenderState St var_buffer 3, (senderOut_Ds (Msg (Pair (last var_buffer) True))))"
   oops
 
 (* Line 24:  St -> Sf [buffer.size()=1] {as==true, i==null} / {buffer=buffer.butlast()}; *)
 lemma transition_5_4:
   assumes "(size var_buffer)=1 \<and> port_as=True"
-    shows "senderTransition ((SenderState St var_buffer var_c), (createSbElem_As_I (Msg port_as) null))
-         = (SenderState Sf (butlast var_buffer) var_c, (tsynbNull (\<C> ''ds'')))"
+    shows "senderTransition ((SenderState St var_buffer var_c), (senderElemIn_As_I (Msg port_as) null))
+         = (SenderState Sf (butlast var_buffer) var_c, (senderOut_Ds null))"
   oops
 
 (* Line 26:  St -> St [buffer.size()=0 && i!=null] {as==null} / {buffer=buffer.prepend(i), c=3, ds=new Pair<>(i,true)}; *)
 lemma transition_6_0:
   assumes "(size var_buffer)=0"
-    shows "senderTransition ((SenderState St var_buffer var_c), (createSbElem_As_I null (Msg port_i)))
-         = (SenderState St (prepend var_buffer port_i) 3, (sbe2SB (createDsBundle (Pair port_i True))))"
+    shows "senderTransition ((SenderState St var_buffer var_c), (senderElemIn_As_I null (Msg port_i)))
+         = (SenderState St (prepend var_buffer port_i) 3, (senderOut_Ds (Msg (Pair port_i True))))"
   oops
 
 (* Line 29:  St -> St [buffer.size()>0 && c>0 && i!=null] {as==null} / {buffer=buffer.prepend(i), c=c-1}; *)
 lemma transition_6_1:
   assumes "(size var_buffer)>0 \<and> var_c>0"
-    shows "senderTransition ((SenderState St var_buffer var_c), (createSbElem_As_I null (Msg port_i)))
-         = (SenderState St (prepend var_buffer port_i) (var_c-1), (tsynbNull (\<C> ''ds'')))"
+    shows "senderTransition ((SenderState St var_buffer var_c), (senderElemIn_As_I null (Msg port_i)))
+         = (SenderState St (prepend var_buffer port_i) (var_c-1), (senderOut_Ds null))"
   oops
 
 (* Line 31:  St -> St [buffer.size()>0 && c=0 && i!=null] {as==null} / {buffer=buffer.prepend(i), c=3, ds=new Pair<>(buffer.last(),true)}; *)
 lemma transition_6_2:
   assumes "(size var_buffer)>0 \<and> var_c=0"
-    shows "senderTransition ((SenderState St var_buffer var_c), (createSbElem_As_I null (Msg port_i)))
-         = (SenderState St (prepend var_buffer port_i) 3, (sbe2SB (createDsBundle (Pair (last var_buffer) True))))"
+    shows "senderTransition ((SenderState St var_buffer var_c), (senderElemIn_As_I null (Msg port_i)))
+         = (SenderState St (prepend var_buffer port_i) 3, (senderOut_Ds (Msg (Pair (last var_buffer) True))))"
   oops
 
 (* Line 19:  St -> St [buffer.size()=0] {as==null, i==null}; *)
 lemma transition_7_0:
   assumes "(size var_buffer)=0"
-    shows "senderTransition ((SenderState St var_buffer var_c), (createSbElem_As_I null null))
-         = (SenderState St var_buffer var_c, (tsynbNull (\<C> ''ds'')))"
+    shows "senderTransition ((SenderState St var_buffer var_c), (senderElemIn_As_I null null))
+         = (SenderState St var_buffer var_c, (senderOut_Ds null))"
   oops
 
 (* Line 21:  St -> St [buffer.size()>0 && c>0] {as==null, i==null} / {c=c-1}; *)
 lemma transition_7_1:
   assumes "(size var_buffer)>0 \<and> var_c>0"
-    shows "senderTransition ((SenderState St var_buffer var_c), (createSbElem_As_I null null))
-         = (SenderState St var_buffer (var_c-1), (tsynbNull (\<C> ''ds'')))"
+    shows "senderTransition ((SenderState St var_buffer var_c), (senderElemIn_As_I null null))
+         = (SenderState St var_buffer (var_c-1), (senderOut_Ds null))"
   oops
 
 (* Line 23:  St -> St [buffer.size()>0 && c=0] {as==null, i==null} / {c=3, ds=new Pair<>(buffer.last(),true)}; *)
 lemma transition_7_2:
   assumes "(size var_buffer)>0 \<and> var_c=0"
-    shows "senderTransition ((SenderState St var_buffer var_c), (createSbElem_As_I null null))
-         = (SenderState St var_buffer 3, (sbe2SB (createDsBundle (Pair (last var_buffer) True))))"
+    shows "senderTransition ((SenderState St var_buffer var_c), (senderElemIn_As_I null null))
+         = (SenderState St var_buffer 3, (senderOut_Ds (Msg (Pair (last var_buffer) True))))"
   oops
 
 
@@ -547,225 +500,225 @@ section \<open>Step-wise lemmata for the SPF\<close>
 (* Line 33:  Sf -> St [buffer.size()>1 && i!=null] {as==false} / {buffer=buffer.butlast().prepend(i), c=3, ds=new Pair<>(buffer.butlast().last(),true)}; *)
 lemma step_0_0:
   assumes "(size var_buffer)>1 \<and> port_as=False"
-    shows "spfConcIn  (createBundle_As_I (Msg port_as) (Msg port_i))\<cdot>(da_h SenderAutomaton (SenderState Sf var_buffer var_c))
-         = spfConcOut (sbe2SB (createDsBundle (Pair (last (butlast var_buffer)) True)))\<cdot>(da_h SenderAutomaton (SenderState St (prepend (butlast var_buffer) port_i) 3))"
+    shows "spfConcIn  (senderIn_As_I (Msg port_as) (Msg port_i))\<cdot>(SenderStep (SenderState Sf var_buffer var_c))
+         = spfConcOut (senderOut_Ds (Msg (Pair (last (butlast var_buffer)) True)))\<cdot>(SenderStep (SenderState St (prepend (butlast var_buffer) port_i) 3))"
   oops
 
 (* Line 35:  Sf -> St [buffer.size()=1 && i!=null] {as==false} / {buffer=buffer.butlast().prepend(i), c=3, ds=new Pair<>(i,true)}; *)
 lemma step_0_1:
   assumes "(size var_buffer)=1 \<and> port_as=False"
-    shows "spfConcIn  (createBundle_As_I (Msg port_as) (Msg port_i))\<cdot>(da_h SenderAutomaton (SenderState Sf var_buffer var_c))
-         = spfConcOut (sbe2SB (createDsBundle (Pair port_i True)))\<cdot>(da_h SenderAutomaton (SenderState St (prepend (butlast var_buffer) port_i) 3))"
+    shows "spfConcIn  (senderIn_As_I (Msg port_as) (Msg port_i))\<cdot>(SenderStep (SenderState Sf var_buffer var_c))
+         = spfConcOut (senderOut_Ds (Msg (Pair port_i True)))\<cdot>(SenderStep (SenderState St (prepend (butlast var_buffer) port_i) 3))"
   oops
 
 (* Line 43:  Sf -> Sf [buffer.size()=0 && as!=null && i!=null] / {buffer=buffer.prepend(i), c=3, ds=new Pair<>(i,false)}; *)
 lemma step_0_2:
   assumes "(size var_buffer)=0"
-    shows "spfConcIn  (createBundle_As_I (Msg port_as) (Msg port_i))\<cdot>(da_h SenderAutomaton (SenderState Sf var_buffer var_c))
-         = spfConcOut (sbe2SB (createDsBundle (Pair port_i False)))\<cdot>(da_h SenderAutomaton (SenderState Sf (prepend var_buffer port_i) 3))"
+    shows "spfConcIn  (senderIn_As_I (Msg port_as) (Msg port_i))\<cdot>(SenderStep (SenderState Sf var_buffer var_c))
+         = spfConcOut (senderOut_Ds (Msg (Pair port_i False)))\<cdot>(SenderStep (SenderState Sf (prepend var_buffer port_i) 3))"
   oops
 
 (* Line 45:  Sf -> Sf [buffer.size()>0 && c>0 && i!=null] {as==true} / {buffer=buffer.prepend(i), c=c-1}; *)
 lemma step_0_3:
   assumes "(size var_buffer)>0 \<and> var_c>0 \<and> port_as=True"
-    shows "spfConcIn  (createBundle_As_I (Msg port_as) (Msg port_i))\<cdot>(da_h SenderAutomaton (SenderState Sf var_buffer var_c))
-         = spfConcOut (tsynbNull (\<C> ''ds''))\<cdot>(da_h SenderAutomaton (SenderState Sf (prepend var_buffer port_i) (var_c-1)))"
+    shows "spfConcIn  (senderIn_As_I (Msg port_as) (Msg port_i))\<cdot>(SenderStep (SenderState Sf var_buffer var_c))
+         = spfConcOut (senderOut_Ds null)\<cdot>(SenderStep (SenderState Sf (prepend var_buffer port_i) (var_c-1)))"
   oops
 
 (* Line 47:  Sf -> Sf [buffer.size()>0 && c=0 && i!=null] {as==true} / {buffer=buffer.prepend(i), c=3, ds=new Pair<>(buffer.last(),false)}; *)
 lemma step_0_4:
   assumes "(size var_buffer)>0 \<and> var_c=0 \<and> port_as=True"
-    shows "spfConcIn  (createBundle_As_I (Msg port_as) (Msg port_i))\<cdot>(da_h SenderAutomaton (SenderState Sf var_buffer var_c))
-         = spfConcOut (sbe2SB (createDsBundle (Pair (last var_buffer) False)))\<cdot>(da_h SenderAutomaton (SenderState Sf (prepend var_buffer port_i) 3))"
+    shows "spfConcIn  (senderIn_As_I (Msg port_as) (Msg port_i))\<cdot>(SenderStep (SenderState Sf var_buffer var_c))
+         = spfConcOut (senderOut_Ds (Msg (Pair (last var_buffer) False)))\<cdot>(SenderStep (SenderState Sf (prepend var_buffer port_i) 3))"
   oops
 
 (* Line 34:  Sf -> St [buffer.size()>1] {as==false, i==null} / {buffer=buffer.butlast(), c=3, ds=new Pair<>(buffer.butlast().last(),true)}; *)
 lemma step_1_0:
   assumes "(size var_buffer)>1 \<and> port_as=False"
-    shows "spfConcIn  (createBundle_As_I (Msg port_as) null)\<cdot>(da_h SenderAutomaton (SenderState Sf var_buffer var_c))
-         = spfConcOut (sbe2SB (createDsBundle (Pair (last (butlast var_buffer)) True)))\<cdot>(da_h SenderAutomaton (SenderState St (butlast var_buffer) 3))"
+    shows "spfConcIn  (senderIn_As_I (Msg port_as) null)\<cdot>(SenderStep (SenderState Sf var_buffer var_c))
+         = spfConcOut (senderOut_Ds (Msg (Pair (last (butlast var_buffer)) True)))\<cdot>(SenderStep (SenderState St (butlast var_buffer) 3))"
   oops
 
 (* Line 36:  Sf -> St [buffer.size()=1] {as==false, i==null} / {buffer=buffer.butlast()}; *)
 lemma step_1_1:
   assumes "(size var_buffer)=1 \<and> port_as=False"
-    shows "spfConcIn  (createBundle_As_I (Msg port_as) null)\<cdot>(da_h SenderAutomaton (SenderState Sf var_buffer var_c))
-         = spfConcOut (tsynbNull (\<C> ''ds''))\<cdot>(da_h SenderAutomaton (SenderState St (butlast var_buffer) var_c))"
+    shows "spfConcIn  (senderIn_As_I (Msg port_as) null)\<cdot>(SenderStep (SenderState Sf var_buffer var_c))
+         = spfConcOut (senderOut_Ds null)\<cdot>(SenderStep (SenderState St (butlast var_buffer) var_c))"
   oops
 
 (* Line 38:  Sf -> Sf [buffer.size()=0 && as!=null] {i==null}; *)
 lemma step_1_2:
   assumes "(size var_buffer)=0"
-    shows "spfConcIn  (createBundle_As_I (Msg port_as) null)\<cdot>(da_h SenderAutomaton (SenderState Sf var_buffer var_c))
-         = spfConcOut (tsynbNull (\<C> ''ds''))\<cdot>(da_h SenderAutomaton (SenderState Sf var_buffer var_c))"
+    shows "spfConcIn  (senderIn_As_I (Msg port_as) null)\<cdot>(SenderStep (SenderState Sf var_buffer var_c))
+         = spfConcOut (senderOut_Ds null)\<cdot>(SenderStep (SenderState Sf var_buffer var_c))"
   oops
 
 (* Line 40:  Sf -> Sf [buffer.size()>0 && c>0] {as==true, i==null} / {c=c-1}; *)
 lemma step_1_3:
   assumes "(size var_buffer)>0 \<and> var_c>0 \<and> port_as=True"
-    shows "spfConcIn  (createBundle_As_I (Msg port_as) null)\<cdot>(da_h SenderAutomaton (SenderState Sf var_buffer var_c))
-         = spfConcOut (tsynbNull (\<C> ''ds''))\<cdot>(da_h SenderAutomaton (SenderState Sf var_buffer (var_c-1)))"
+    shows "spfConcIn  (senderIn_As_I (Msg port_as) null)\<cdot>(SenderStep (SenderState Sf var_buffer var_c))
+         = spfConcOut (senderOut_Ds null)\<cdot>(SenderStep (SenderState Sf var_buffer (var_c-1)))"
   oops
 
 (* Line 41:  Sf -> Sf [buffer.size()>0 && c=0] {as==true, i==null} / {c=3, ds=new Pair<>(buffer.last(),false)}; *)
 lemma step_1_4:
   assumes "(size var_buffer)>0 \<and> var_c=0 \<and> port_as=True"
-    shows "spfConcIn  (createBundle_As_I (Msg port_as) null)\<cdot>(da_h SenderAutomaton (SenderState Sf var_buffer var_c))
-         = spfConcOut (sbe2SB (createDsBundle (Pair (last var_buffer) False)))\<cdot>(da_h SenderAutomaton (SenderState Sf var_buffer 3))"
+    shows "spfConcIn  (senderIn_As_I (Msg port_as) null)\<cdot>(SenderStep (SenderState Sf var_buffer var_c))
+         = spfConcOut (senderOut_Ds (Msg (Pair (last var_buffer) False)))\<cdot>(SenderStep (SenderState Sf var_buffer 3))"
   oops
 
 (* Line 44:  Sf -> Sf [buffer.size()=0 && i!=null] {as==null} / {buffer=buffer.prepend(i), c=3, ds=new Pair<>(i,false)}; *)
 lemma step_2_0:
   assumes "(size var_buffer)=0"
-    shows "spfConcIn  (createBundle_As_I null (Msg port_i))\<cdot>(da_h SenderAutomaton (SenderState Sf var_buffer var_c))
-         = spfConcOut (sbe2SB (createDsBundle (Pair port_i False)))\<cdot>(da_h SenderAutomaton (SenderState Sf (prepend var_buffer port_i) 3))"
+    shows "spfConcIn  (senderIn_As_I null (Msg port_i))\<cdot>(SenderStep (SenderState Sf var_buffer var_c))
+         = spfConcOut (senderOut_Ds (Msg (Pair port_i False)))\<cdot>(SenderStep (SenderState Sf (prepend var_buffer port_i) 3))"
   oops
 
 (* Line 46:  Sf -> Sf [buffer.size()>0 && c>0 && i!=null] {as==null} / {buffer=buffer.prepend(i), c=c-1}; *)
 lemma step_2_1:
   assumes "(size var_buffer)>0 \<and> var_c>0"
-    shows "spfConcIn  (createBundle_As_I null (Msg port_i))\<cdot>(da_h SenderAutomaton (SenderState Sf var_buffer var_c))
-         = spfConcOut (tsynbNull (\<C> ''ds''))\<cdot>(da_h SenderAutomaton (SenderState Sf (prepend var_buffer port_i) (var_c-1)))"
+    shows "spfConcIn  (senderIn_As_I null (Msg port_i))\<cdot>(SenderStep (SenderState Sf var_buffer var_c))
+         = spfConcOut (senderOut_Ds null)\<cdot>(SenderStep (SenderState Sf (prepend var_buffer port_i) (var_c-1)))"
   oops
 
 (* Line 48:  Sf -> Sf [buffer.size()>0 && c=0 && i!=null] {as==null} / {buffer=buffer.prepend(i), c=3, ds=new Pair<>(buffer.last(),false)}; *)
 lemma step_2_2:
   assumes "(size var_buffer)>0 \<and> var_c=0"
-    shows "spfConcIn  (createBundle_As_I null (Msg port_i))\<cdot>(da_h SenderAutomaton (SenderState Sf var_buffer var_c))
-         = spfConcOut (sbe2SB (createDsBundle (Pair (last var_buffer) False)))\<cdot>(da_h SenderAutomaton (SenderState Sf (prepend var_buffer port_i) 3))"
+    shows "spfConcIn  (senderIn_As_I null (Msg port_i))\<cdot>(SenderStep (SenderState Sf var_buffer var_c))
+         = spfConcOut (senderOut_Ds (Msg (Pair (last var_buffer) False)))\<cdot>(SenderStep (SenderState Sf (prepend var_buffer port_i) 3))"
   oops
 
 (* Line 37:  Sf -> Sf [buffer.size()=0] {as==null, i==null}; *)
 lemma step_3_0:
   assumes "(size var_buffer)=0"
-    shows "spfConcIn  (createBundle_As_I null null)\<cdot>(da_h SenderAutomaton (SenderState Sf var_buffer var_c))
-         = spfConcOut (tsynbNull (\<C> ''ds''))\<cdot>(da_h SenderAutomaton (SenderState Sf var_buffer var_c))"
+    shows "spfConcIn  (senderIn_As_I null null)\<cdot>(SenderStep (SenderState Sf var_buffer var_c))
+         = spfConcOut (senderOut_Ds null)\<cdot>(SenderStep (SenderState Sf var_buffer var_c))"
   oops
 
 (* Line 39:  Sf -> Sf [buffer.size()>0 && c>0] {as==null, i==null}; *)
 lemma step_3_1:
   assumes "(size var_buffer)>0 \<and> var_c>0"
-    shows "spfConcIn  (createBundle_As_I null null)\<cdot>(da_h SenderAutomaton (SenderState Sf var_buffer var_c))
-         = spfConcOut (tsynbNull (\<C> ''ds''))\<cdot>(da_h SenderAutomaton (SenderState Sf var_buffer var_c))"
+    shows "spfConcIn  (senderIn_As_I null null)\<cdot>(SenderStep (SenderState Sf var_buffer var_c))
+         = spfConcOut (senderOut_Ds null)\<cdot>(SenderStep (SenderState Sf var_buffer var_c))"
   oops
 
 (* Line 42:  Sf -> Sf [buffer.size()>0 && c=0] {as==null, i==null} / {c=3, ds=new Pair<>(buffer.last(),false)}; *)
 lemma step_3_2:
   assumes "(size var_buffer)>0 \<and> var_c=0"
-    shows "spfConcIn  (createBundle_As_I null null)\<cdot>(da_h SenderAutomaton (SenderState Sf var_buffer var_c))
-         = spfConcOut (sbe2SB (createDsBundle (Pair (last var_buffer) False)))\<cdot>(da_h SenderAutomaton (SenderState Sf var_buffer 3))"
+    shows "spfConcIn  (senderIn_As_I null null)\<cdot>(SenderStep (SenderState Sf var_buffer var_c))
+         = spfConcOut (senderOut_Ds (Msg (Pair (last var_buffer) False)))\<cdot>(SenderStep (SenderState Sf var_buffer 3))"
   oops
 
 (* Line 25:  St -> St [buffer.size()=0 && as!=null && i!=null] / {buffer=buffer.prepend(i), c=3, ds=new Pair<>(i,true)}; *)
 lemma step_4_0:
   assumes "(size var_buffer)=0"
-    shows "spfConcIn  (createBundle_As_I (Msg port_as) (Msg port_i))\<cdot>(da_h SenderAutomaton (SenderState St var_buffer var_c))
-         = spfConcOut (sbe2SB (createDsBundle (Pair port_i True)))\<cdot>(da_h SenderAutomaton (SenderState St (prepend var_buffer port_i) 3))"
+    shows "spfConcIn  (senderIn_As_I (Msg port_as) (Msg port_i))\<cdot>(SenderStep (SenderState St var_buffer var_c))
+         = spfConcOut (senderOut_Ds (Msg (Pair port_i True)))\<cdot>(SenderStep (SenderState St (prepend var_buffer port_i) 3))"
   oops
 
 (* Line 27:  St -> Sf [buffer.size()>1 && i!=null] {as==true} / {buffer=buffer.butlast().prepend(i), c=3, ds=new Pair<>(buffer.butlast().last(),false)}; *)
 lemma step_4_1:
   assumes "(size var_buffer)>1 \<and> port_as=True"
-    shows "spfConcIn  (createBundle_As_I (Msg port_as) (Msg port_i))\<cdot>(da_h SenderAutomaton (SenderState St var_buffer var_c))
-         = spfConcOut (sbe2SB (createDsBundle (Pair (last (butlast var_buffer)) False)))\<cdot>(da_h SenderAutomaton (SenderState Sf (prepend (butlast var_buffer) port_i) 3))"
+    shows "spfConcIn  (senderIn_As_I (Msg port_as) (Msg port_i))\<cdot>(SenderStep (SenderState St var_buffer var_c))
+         = spfConcOut (senderOut_Ds (Msg (Pair (last (butlast var_buffer)) False)))\<cdot>(SenderStep (SenderState Sf (prepend (butlast var_buffer) port_i) 3))"
   oops
 
 (* Line 28:  St -> St [buffer.size()>0 && c>0 && i!=null] {as==false} / {buffer=buffer.prepend(i), c=c-1}; *)
 lemma step_4_2:
   assumes "(size var_buffer)>0 \<and> var_c>0 \<and> port_as=False"
-    shows "spfConcIn  (createBundle_As_I (Msg port_as) (Msg port_i))\<cdot>(da_h SenderAutomaton (SenderState St var_buffer var_c))
-         = spfConcOut (tsynbNull (\<C> ''ds''))\<cdot>(da_h SenderAutomaton (SenderState St (prepend var_buffer port_i) (var_c-1)))"
+    shows "spfConcIn  (senderIn_As_I (Msg port_as) (Msg port_i))\<cdot>(SenderStep (SenderState St var_buffer var_c))
+         = spfConcOut (senderOut_Ds null)\<cdot>(SenderStep (SenderState St (prepend var_buffer port_i) (var_c-1)))"
   oops
 
 (* Line 30:  St -> St [buffer.size()>0 && c=0 && i!=null] {as==false} / {buffer=buffer.prepend(i), c=3, ds=new Pair<>(buffer.last(),true)}; *)
 lemma step_4_3:
   assumes "(size var_buffer)>0 \<and> var_c=0 \<and> port_as=False"
-    shows "spfConcIn  (createBundle_As_I (Msg port_as) (Msg port_i))\<cdot>(da_h SenderAutomaton (SenderState St var_buffer var_c))
-         = spfConcOut (sbe2SB (createDsBundle (Pair (last var_buffer) True)))\<cdot>(da_h SenderAutomaton (SenderState St (prepend var_buffer port_i) 3))"
+    shows "spfConcIn  (senderIn_As_I (Msg port_as) (Msg port_i))\<cdot>(SenderStep (SenderState St var_buffer var_c))
+         = spfConcOut (senderOut_Ds (Msg (Pair (last var_buffer) True)))\<cdot>(SenderStep (SenderState St (prepend var_buffer port_i) 3))"
   oops
 
 (* Line 32:  St -> Sf [buffer.size()=1 && i!=null] {as==true} / {buffer=buffer.butlast().prepend(i), c=3, ds=new Pair<>(i,false)}; *)
 lemma step_4_4:
   assumes "(size var_buffer)=1 \<and> port_as=True"
-    shows "spfConcIn  (createBundle_As_I (Msg port_as) (Msg port_i))\<cdot>(da_h SenderAutomaton (SenderState St var_buffer var_c))
-         = spfConcOut (sbe2SB (createDsBundle (Pair port_i False)))\<cdot>(da_h SenderAutomaton (SenderState Sf (prepend (butlast var_buffer) port_i) 3))"
+    shows "spfConcIn  (senderIn_As_I (Msg port_as) (Msg port_i))\<cdot>(SenderStep (SenderState St var_buffer var_c))
+         = spfConcOut (senderOut_Ds (Msg (Pair port_i False)))\<cdot>(SenderStep (SenderState Sf (prepend (butlast var_buffer) port_i) 3))"
   oops
 
 (* Line 17:  St -> St [buffer.size()=0 && as!=null] {i==null}; *)
 lemma step_5_0:
   assumes "(size var_buffer)=0"
-    shows "spfConcIn  (createBundle_As_I (Msg port_as) null)\<cdot>(da_h SenderAutomaton (SenderState St var_buffer var_c))
-         = spfConcOut (tsynbNull (\<C> ''ds''))\<cdot>(da_h SenderAutomaton (SenderState St var_buffer var_c))"
+    shows "spfConcIn  (senderIn_As_I (Msg port_as) null)\<cdot>(SenderStep (SenderState St var_buffer var_c))
+         = spfConcOut (senderOut_Ds null)\<cdot>(SenderStep (SenderState St var_buffer var_c))"
   oops
 
 (* Line 18:  St -> Sf [buffer.size()>1] {as==true, i==null} / {buffer=buffer.butlast(), c=3, ds=new Pair<>(buffer.butlast().last(),false)}; *)
 lemma step_5_1:
   assumes "(size var_buffer)>1 \<and> port_as=True"
-    shows "spfConcIn  (createBundle_As_I (Msg port_as) null)\<cdot>(da_h SenderAutomaton (SenderState St var_buffer var_c))
-         = spfConcOut (sbe2SB (createDsBundle (Pair (last (butlast var_buffer)) False)))\<cdot>(da_h SenderAutomaton (SenderState Sf (butlast var_buffer) 3))"
+    shows "spfConcIn  (senderIn_As_I (Msg port_as) null)\<cdot>(SenderStep (SenderState St var_buffer var_c))
+         = spfConcOut (senderOut_Ds (Msg (Pair (last (butlast var_buffer)) False)))\<cdot>(SenderStep (SenderState Sf (butlast var_buffer) 3))"
   oops
 
 (* Line 20:  St -> St [buffer.size()>0 && c>0] {as==false, i==null} / {c=c-1}; *)
 lemma step_5_2:
   assumes "(size var_buffer)>0 \<and> var_c>0 \<and> port_as=False"
-    shows "spfConcIn  (createBundle_As_I (Msg port_as) null)\<cdot>(da_h SenderAutomaton (SenderState St var_buffer var_c))
-         = spfConcOut (tsynbNull (\<C> ''ds''))\<cdot>(da_h SenderAutomaton (SenderState St var_buffer (var_c-1)))"
+    shows "spfConcIn  (senderIn_As_I (Msg port_as) null)\<cdot>(SenderStep (SenderState St var_buffer var_c))
+         = spfConcOut (senderOut_Ds null)\<cdot>(SenderStep (SenderState St var_buffer (var_c-1)))"
   oops
 
 (* Line 22:  St -> St [buffer.size()>0 && c=0] {as==false, i==null} / {c=3, ds=new Pair<>(buffer.last(),true)}; *)
 lemma step_5_3:
   assumes "(size var_buffer)>0 \<and> var_c=0 \<and> port_as=False"
-    shows "spfConcIn  (createBundle_As_I (Msg port_as) null)\<cdot>(da_h SenderAutomaton (SenderState St var_buffer var_c))
-         = spfConcOut (sbe2SB (createDsBundle (Pair (last var_buffer) True)))\<cdot>(da_h SenderAutomaton (SenderState St var_buffer 3))"
+    shows "spfConcIn  (senderIn_As_I (Msg port_as) null)\<cdot>(SenderStep (SenderState St var_buffer var_c))
+         = spfConcOut (senderOut_Ds (Msg (Pair (last var_buffer) True)))\<cdot>(SenderStep (SenderState St var_buffer 3))"
   oops
 
 (* Line 24:  St -> Sf [buffer.size()=1] {as==true, i==null} / {buffer=buffer.butlast()}; *)
 lemma step_5_4:
   assumes "(size var_buffer)=1 \<and> port_as=True"
-    shows "spfConcIn  (createBundle_As_I (Msg port_as) null)\<cdot>(da_h SenderAutomaton (SenderState St var_buffer var_c))
-         = spfConcOut (tsynbNull (\<C> ''ds''))\<cdot>(da_h SenderAutomaton (SenderState Sf (butlast var_buffer) var_c))"
+    shows "spfConcIn  (senderIn_As_I (Msg port_as) null)\<cdot>(SenderStep (SenderState St var_buffer var_c))
+         = spfConcOut (senderOut_Ds null)\<cdot>(SenderStep (SenderState Sf (butlast var_buffer) var_c))"
   oops
 
 (* Line 26:  St -> St [buffer.size()=0 && i!=null] {as==null} / {buffer=buffer.prepend(i), c=3, ds=new Pair<>(i,true)}; *)
 lemma step_6_0:
   assumes "(size var_buffer)=0"
-    shows "spfConcIn  (createBundle_As_I null (Msg port_i))\<cdot>(da_h SenderAutomaton (SenderState St var_buffer var_c))
-         = spfConcOut (sbe2SB (createDsBundle (Pair port_i True)))\<cdot>(da_h SenderAutomaton (SenderState St (prepend var_buffer port_i) 3))"
+    shows "spfConcIn  (senderIn_As_I null (Msg port_i))\<cdot>(SenderStep (SenderState St var_buffer var_c))
+         = spfConcOut (senderOut_Ds (Msg (Pair port_i True)))\<cdot>(SenderStep (SenderState St (prepend var_buffer port_i) 3))"
   oops
 
 (* Line 29:  St -> St [buffer.size()>0 && c>0 && i!=null] {as==null} / {buffer=buffer.prepend(i), c=c-1}; *)
 lemma step_6_1:
   assumes "(size var_buffer)>0 \<and> var_c>0"
-    shows "spfConcIn  (createBundle_As_I null (Msg port_i))\<cdot>(da_h SenderAutomaton (SenderState St var_buffer var_c))
-         = spfConcOut (tsynbNull (\<C> ''ds''))\<cdot>(da_h SenderAutomaton (SenderState St (prepend var_buffer port_i) (var_c-1)))"
+    shows "spfConcIn  (senderIn_As_I null (Msg port_i))\<cdot>(SenderStep (SenderState St var_buffer var_c))
+         = spfConcOut (senderOut_Ds null)\<cdot>(SenderStep (SenderState St (prepend var_buffer port_i) (var_c-1)))"
   oops
 
 (* Line 31:  St -> St [buffer.size()>0 && c=0 && i!=null] {as==null} / {buffer=buffer.prepend(i), c=3, ds=new Pair<>(buffer.last(),true)}; *)
 lemma step_6_2:
   assumes "(size var_buffer)>0 \<and> var_c=0"
-    shows "spfConcIn  (createBundle_As_I null (Msg port_i))\<cdot>(da_h SenderAutomaton (SenderState St var_buffer var_c))
-         = spfConcOut (sbe2SB (createDsBundle (Pair (last var_buffer) True)))\<cdot>(da_h SenderAutomaton (SenderState St (prepend var_buffer port_i) 3))"
+    shows "spfConcIn  (senderIn_As_I null (Msg port_i))\<cdot>(SenderStep (SenderState St var_buffer var_c))
+         = spfConcOut (senderOut_Ds (Msg (Pair (last var_buffer) True)))\<cdot>(SenderStep (SenderState St (prepend var_buffer port_i) 3))"
   oops
 
 (* Line 19:  St -> St [buffer.size()=0] {as==null, i==null}; *)
 lemma step_7_0:
   assumes "(size var_buffer)=0"
-    shows "spfConcIn  (createBundle_As_I null null)\<cdot>(da_h SenderAutomaton (SenderState St var_buffer var_c))
-         = spfConcOut (tsynbNull (\<C> ''ds''))\<cdot>(da_h SenderAutomaton (SenderState St var_buffer var_c))"
+    shows "spfConcIn  (senderIn_As_I null null)\<cdot>(SenderStep (SenderState St var_buffer var_c))
+         = spfConcOut (senderOut_Ds null)\<cdot>(SenderStep (SenderState St var_buffer var_c))"
   oops
 
 (* Line 21:  St -> St [buffer.size()>0 && c>0] {as==null, i==null} / {c=c-1}; *)
 lemma step_7_1:
   assumes "(size var_buffer)>0 \<and> var_c>0"
-    shows "spfConcIn  (createBundle_As_I null null)\<cdot>(da_h SenderAutomaton (SenderState St var_buffer var_c))
-         = spfConcOut (tsynbNull (\<C> ''ds''))\<cdot>(da_h SenderAutomaton (SenderState St var_buffer (var_c-1)))"
+    shows "spfConcIn  (senderIn_As_I null null)\<cdot>(SenderStep (SenderState St var_buffer var_c))
+         = spfConcOut (senderOut_Ds null)\<cdot>(SenderStep (SenderState St var_buffer (var_c-1)))"
   oops
 
 (* Line 23:  St -> St [buffer.size()>0 && c=0] {as==null, i==null} / {c=3, ds=new Pair<>(buffer.last(),true)}; *)
 lemma step_7_2:
   assumes "(size var_buffer)>0 \<and> var_c=0"
-    shows "spfConcIn  (createBundle_As_I null null)\<cdot>(da_h SenderAutomaton (SenderState St var_buffer var_c))
-         = spfConcOut (sbe2SB (createDsBundle (Pair (last var_buffer) True)))\<cdot>(da_h SenderAutomaton (SenderState St var_buffer 3))"
+    shows "spfConcIn  (senderIn_As_I null null)\<cdot>(SenderStep (SenderState St var_buffer var_c))
+         = spfConcOut (senderOut_Ds (Msg (Pair (last var_buffer) True)))\<cdot>(SenderStep (SenderState St var_buffer 3))"
   oops
 
 
